undo moving of postcondition and clean up UnsaturatedSolinas interface

src/Bedrock/UnsaturatedSolinas.v
@@ -59,7 +59,27 @@ Section __.
           {inname_gen outname_gen : nat -> string}
           (n : nat) (s : Z) (c : list (Z * Z)).
   Context (carry_mul_name add_name to_bytes_name : string).
+  Local Notation loose_bounds := (UnsaturatedSolinas.loose_bounds n s c).
+  Local Notation tight_bounds := (UnsaturatedSolinas.tight_bounds n s c).
+  Local Notation M := (s - Associational.eval c)%Z.
+  Definition weight :=
+    (ModOps.weight
+       (Qnum (inject_Z (Z.log2_up M) / inject_Z (Z.of_nat n)))
+       (QDen (inject_Z (Z.log2_up M) / inject_Z (Z.of_nat n)))).
+  Local Notation eval := (eval weight n).
 
+  (* for to/from bytes *)
+  Local Definition limbwidth :=
+    (Z.log2_up (s - Associational.eval c) / Z.of_nat n)%Q.
+  Local Definition n_bytes :=
+    (Freeze.bytes_n (Qnum limbwidth) (Qden limbwidth) n).
+  Let prime_bytes_upperbound_list :=
+    encode_no_reduce (ModOps.weight 8 1) n_bytes (s - 1).
+  Let prime_bytes_bounds :=
+    map (fun v : Z => Some {| ZRange.lower := 0; ZRange.upper := v |})
+        prime_bytes_upperbound_list.
+
+  (* convenience notation for readability *)
   Local Notation foreach_arg F t :=
     (type.for_each_lhs_of_arrow F t) (only parsing).
   Local Notation foreach_ret F t :=
@@ -74,67 +94,279 @@ Section __.
                         (make_outnames (outname_gen:=outname_gen) _)
                         outsizes).
 
-  Record FunctionSignature t :=
+  Record operation (t : API.type) :=
     { name : string;
+      inbounds : foreach_arg ZRange.type.option.interp t;
       input_array_sizes : foreach_arg access_sizes t;
       output_array_sizes : foreach_ret access_sizes t;
       input_array_lengths : foreach_arg list_lengths t;
       output_array_lengths : foreach_ret list_lengths t;
+      pipeline_out : Pipeline.ErrorT (API.Expr t);
+      postcondition : foreach_arg API.interp_type t
+                      -> foreach_ret API.interp_type t -> Prop;
+      correctness :
+        check_args
+          n s c Semantics.width (ErrorT.Success tt) = ErrorT.Success tt ->
+        forall res,
+          pipeline_out = ErrorT.Success res ->
+          forall args,
+            postcondition args (type.app_curried (API.Interp res) args)
     }.
   Arguments name {_}.
+  Arguments inbounds {_}.
   Arguments input_array_sizes {_}.
   Arguments output_array_sizes {_}.
   Arguments input_array_lengths {_}.
   Arguments output_array_lengths {_}.
+  Arguments pipeline_out {_}.
+  Arguments postcondition {_}.
+  Arguments correctness {_}.
 
   Definition make_bedrock_func
-             {t} (sig : FunctionSignature t) (res : API.Expr t)
+             {t} (op : operation t) (res : API.Expr t)
     : bedrock_func :=
-    (sig.(name), make_bedrock_func_with_sizes
-                   (sig.(input_array_sizes)) (sig.(output_array_sizes))
-                   (sig.(input_array_lengths)) res).
+    (op.(name), make_bedrock_func_with_sizes
+                  (op.(input_array_sizes)) (op.(output_array_sizes))
+                  (op.(input_array_lengths)) res).
+
+  Ltac select_access_size bounds :=
+    lazymatch bounds with
+    | Some loose_bounds => constr:(access_size.word)
+    | Some tight_bounds => constr:(access_size.word)
+    | Some prime_bytes_bounds => constr:(access_size.one)
+    | ?b => fail "unable to select access size for bound " b
+    end.
+
+  Ltac sizes_from_bounds bounds :=
+    lazymatch bounds with
+    | (?a, ?b) =>
+      let x := sizes_from_bounds a in
+      let y := sizes_from_bounds b in
+      constr:((x, y))
+    | tt => constr:(tt)
+    | ?b => lazymatch type of b with
+            | option (list _) => select_access_size b
+            | _ => constr:(tt)
+            end
+    end.
+
+  Ltac select_length bounds :=
+    lazymatch bounds with
+    | Some loose_bounds => constr:(n)
+    | Some tight_bounds => constr:(n)
+    | Some prime_bytes_bounds => constr:(n_bytes)
+    | ?b => fail "unable to select array length for bound " b
+    end.
+
+  Ltac lengths_from_bounds bounds :=
+    lazymatch bounds with
+    | (?a, ?b) =>
+      let x := lengths_from_bounds a in
+      let y := lengths_from_bounds b in
+      constr:((x, y))
+    | tt => constr:(tt)
+    | ?b => lazymatch type of b with
+            | option (list _) => select_length b
+            | _ => constr:(tt)
+            end
+    end.
+
+  Ltac apply_correctness_in H :=
+    match type of H with
+    | context [UnsaturatedSolinas.carry_mul] =>
+      apply UnsaturatedSolinas.carry_mul_correct in H
+    | context [UnsaturatedSolinas.add] =>
+      apply UnsaturatedSolinas.add_correct in H
+    | context [UnsaturatedSolinas.sub] =>
+      apply UnsaturatedSolinas.sub_correct in H
+    | context [UnsaturatedSolinas.opp] =>
+      apply UnsaturatedSolinas.opp_correct in H
+    | context [UnsaturatedSolinas.carry] =>
+      apply UnsaturatedSolinas.carry_correct in H
+    | context [UnsaturatedSolinas.encode] =>
+      apply UnsaturatedSolinas.encode_correct in H
+    | context [UnsaturatedSolinas.zero] =>
+      apply UnsaturatedSolinas.zero_correct in H
+    | context [UnsaturatedSolinas.one] =>
+      apply UnsaturatedSolinas.one_correct in H
+    | context [UnsaturatedSolinas.to_bytes] =>
+      apply UnsaturatedSolinas.to_bytes_correct in H
+    | context [UnsaturatedSolinas.from_bytes] =>
+      apply UnsaturatedSolinas.from_bytes_correct in H
+    end.
+  Ltac apply_correctness :=
+    match goal with H : _ = ErrorT.Success _ |- _ =>
+                    apply_correctness_in H;
+                    [ | assumption .. ]
+    end.
+
+  Ltac specialize_to_args Hcorrect :=
+    let A := fresh "A" in
+    let A' := fresh "A" in
+    match goal with
+      a : type.for_each_lhs_of_arrow API.interp_type _ |- _ =>
+      cbn in a; set (A:=a)
+    end;
+    repeat match type of A with
+             (?xt * ?yt)%type =>
+             specialize (Hcorrect (fst A));
+             set (A':=snd A); subst A;
+             rename A' into A
+           end;
+    subst A.
+
+  Ltac postcondition_from_correctness :=
+    cbn [type.app_curried API.interp_type
+                          Language.Compilers.base.interp
+                          Compilers.base_interp] in *;
+  lazymatch goal with
+  | Hcorrect : context [?res] |- ?post ?args ?res =>
+    let T := lazymatch type of Hcorrect with ?T => T end in
+    let F := lazymatch (eval pattern res in T) with
+               ?f _ => f end in
+    let F := lazymatch (eval pattern args in F) with
+               ?f _ => f end in
+    let H := fresh in
+    assert (F args res) as H by exact Hcorrect;
+      exact H
+  end.
+
+  Ltac prove_operation_correctness :=
+    intros;
+    let Hcorrect :=
+        lazymatch goal with H : _ = ErrorT.Success _ |- _ => H end in
+    apply_correctness_in Hcorrect; fold weight in *;
+    specialize_to_args Hcorrect; postcondition_from_correctness.
+
+  Ltac make_operation name inbounds outbounds out :=
+    let t := lazymatch goal with |- operation ?t => t end in
+    let insizes := sizes_from_bounds inbounds in
+    let outsizes := sizes_from_bounds outbounds in
+    let inlengths := lengths_from_bounds inbounds in
+    let outlengths := lengths_from_bounds outbounds in
+    eapply (Build_operation
+              t name inbounds
+              insizes outsizes inlengths outlengths)
+           with (pipeline_out:=out).
 
   Definition carry_mul
-    : FunctionSignature (type_listZ -> type_listZ -> type_listZ) :=
-    {| name := carry_mul_name;
-       input_array_sizes := access_sizes_repeat_args access_size.word _;
-       output_array_sizes := access_sizes_repeat_base access_size.word _;
-       input_array_lengths := list_lengths_repeat_args n _;
-       output_array_lengths := list_lengths_repeat_base n _ |}.
+    : operation (type_listZ -> type_listZ -> type_listZ).
+  Proof.
+    make_operation carry_mul_name
+                   (Some loose_bounds, (Some loose_bounds, tt))
+                   (Some tight_bounds)
+                   (UnsaturatedSolinas.carry_mul n s c Semantics.width).
+    prove_operation_correctness.
+  Defined.
 
   Definition add
-    : FunctionSignature (type_listZ -> type_listZ -> type_listZ) :=
-    {| name := add_name;
-       input_array_sizes := access_sizes_repeat_args access_size.word _;
-       output_array_sizes := access_sizes_repeat_base access_size.word _;
-       input_array_lengths := list_lengths_repeat_args n _;
-       output_array_lengths := list_lengths_repeat_base n _ |}.
-
-  Local Definition limbwidth :=
-    (Z.log2_up (s - Associational.eval c) / Z.of_nat n)%Q.
-  Local Definition n_bytes :=
-    (Freeze.bytes_n (Qnum limbwidth) (Qden limbwidth) n).
+    : operation (type_listZ -> type_listZ -> type_listZ).
+  Proof.
+    make_operation add_name
+                   (Some loose_bounds, (Some loose_bounds, tt))
+                   (Some tight_bounds)
+                   (UnsaturatedSolinas.add n s c Semantics.width).
+    prove_operation_correctness.
+  Defined.
 
   Definition to_bytes
-    : FunctionSignature (type_listZ -> type_listZ) :=
-    {| name := to_bytes_name;
-       input_array_sizes := access_sizes_repeat_args access_size.word _;
-       output_array_sizes := access_sizes_repeat_base access_size.one _;
-       input_array_lengths := list_lengths_repeat_args n _;
-       output_array_lengths := list_lengths_repeat_base n_bytes _ |}.
+    : operation (type_listZ -> type_listZ).
+  Proof.
+    make_operation to_bytes_name
+                   (Some tight_bounds, tt)
+                   (Some prime_bytes_bounds)
+                   (UnsaturatedSolinas.to_bytes n s c Semantics.width).
+    prove_operation_correctness.
+  Defined.
+
+  Definition Bignum
+    : Semantics.word -> list Semantics.word -> Semantics.mem -> Prop :=
+    array scalar (word.of_Z word_size_in_bytes).
+
+  Definition EncodedBignum
+    : Semantics.word -> list Byte.byte -> Semantics.mem -> Prop :=
+    array ptsto (word.of_Z 1).
+
+  Notation BignumSuchThat :=
+    (fun addr ws P =>
+       let xs := map word.unsigned ws in
+       sep (emp (P xs)) (Bignum addr ws)).
+
+  Notation EncodedBignumSuchThat :=
+    (fun addr ws P =>
+       let xs := map Byte.byte.unsigned ws in
+       sep (emp (P xs)) (EncodedBignum addr ws)).
+
+  Declare Scope sep_scope.
+  Local Delimit Scope sep_scope with sep.
+  Local Infix "*" := sep : sep_scope.
+
+  Definition spec_of_carry_mul : spec_of carry_mul_name :=
+    fun functions =>
+      forall wx wy px py pout wold_out t m
+             (Ra Rr : Semantics.mem -> Prop),
+        let args := (map word.unsigned wx, (map word.unsigned wy, tt)) in
+        let X := BignumSuchThat px wx (list_Z_bounded_by loose_bounds) in
+        let Y := BignumSuchThat py wy (list_Z_bounded_by loose_bounds) in
+        let Out := BignumSuchThat pout wold_out (fun l => length l = n) in
+        (X * Y * Ra)%sep m ->
+        (Out * Rr)%sep m ->
+        WeakestPrecondition.call
+          functions carry_mul_name t m
+          (px :: py :: pout :: nil)
+          (fun t' m' rets =>
+             t = t' /\
+             rets = []%list /\
+             exists wout,
+               sep (BignumSuchThat pout wout
+                                   (carry_mul.(postcondition) args))
+                   Rr m').
+
+  Definition spec_of_add : spec_of add_name :=
+    fun functions =>
+      forall wx wy px py pout wold_out t m
+             (Ra Rr : Semantics.mem -> Prop),
+        let args := (map word.unsigned wx, (map word.unsigned wy, tt)) in
+        let X := BignumSuchThat px wx (list_Z_bounded_by tight_bounds) in
+        let Y := BignumSuchThat py wy (list_Z_bounded_by tight_bounds) in
+        let Out := BignumSuchThat pout wold_out (fun l => length l = n) in
+        (X * Y * Ra)%sep m ->
+        (Out * Rr)%sep m ->
+        WeakestPrecondition.call
+          functions add_name t m
+          (px :: py :: pout :: nil)
+          (fun t' m' rets =>
+             t = t' /\
+             rets = []%list /\
+             exists wout,
+               sep (BignumSuchThat pout wout
+                                   (add.(postcondition) args))
+                   Rr m').
+
+  Definition spec_of_to_bytes : spec_of add_name :=
+    fun functions =>
+      forall wx px pout wold_out t m
+             (Ra Rr : Semantics.mem -> Prop),
+        let args := (map word.unsigned wx, tt) in
+        let X := BignumSuchThat px wx (list_Z_bounded_by tight_bounds) in
+        let Out := EncodedBignumSuchThat
+                     pout wold_out (fun l => length l = n_bytes) in
+        (X  * Ra)%sep m ->
+        (Out * Rr)%sep m ->
+        WeakestPrecondition.call
+          functions to_bytes_name t m
+          (px :: pout :: nil)
+          (fun t' m' rets =>
+             t = t' /\
+             rets = []%list /\
+             exists wout,
+               sep (EncodedBignumSuchThat
+                      pout wout (to_bytes.(postcondition) args))
+                   Rr m').
 
   Section Proofs.
     Context {ok : Types.ok}.
     Existing Instance semantics_ok.
-
-    Local Notation M := (s - Associational.eval c)%Z.
-    Definition weight :=
-      (ModOps.weight
-         (Qnum (inject_Z (Z.log2_up M) / inject_Z (Z.of_nat n)))
-         (QDen (inject_Z (Z.log2_up M) / inject_Z (Z.of_nat n)))).
-    Local Notation eval := (eval weight n).
-    Local Notation loose_bounds := (UnsaturatedSolinas.loose_bounds n s c).
-    Local Notation tight_bounds := (UnsaturatedSolinas.tight_bounds n s c).
 
     (* loose_bounds_ok could be proven in parameterized form, but is a pain
       and is easily computable with parameters plugged in. So for now, leaving
@@ -150,24 +382,6 @@ Section __.
             (outname_gen_inname_gen_ok : disjoint outname_gen inname_gen).
     Context (inname_gen_unique : unique inname_gen)
             (outname_gen_unique : unique outname_gen).
-
-    (* TODO : add length to Bignums and ByteArrays *)
-    Definition Bignum : Semantics.word -> list Semantics.word -> Semantics.mem -> Prop :=
-      array scalar (word.of_Z word_size_in_bytes).
-
-    Definition EncodedBignum
-      : Semantics.word -> list Byte.byte -> Semantics.mem -> Prop :=
-      array ptsto (word.of_Z 1).
-
-    Notation BignumSuchThat :=
-      (fun addr ws P =>
-         let xs := map word.unsigned ws in
-         sep (emp (P xs)) (Bignum addr ws)).
-
-    Notation EncodedBignumSuchThat :=
-      (fun addr ws P =>
-         let xs := map Byte.byte.unsigned ws in
-         sep (emp (P xs)) (EncodedBignum addr ws)).
 
     Lemma Bignum_of_bytes addr bs :
       length bs = (n * Z.to_nat word_size_in_bytes)%nat ->
@@ -254,273 +468,53 @@ Section __.
                 apply relax_to_max_bounds; apply H ]
       end.
 
-    Ltac apply_correctness_in H :=
-      match type of H with
-      | context [UnsaturatedSolinas.carry_mul] =>
-        apply UnsaturatedSolinas.carry_mul_correct in H
-      | context [UnsaturatedSolinas.add] =>
-        apply UnsaturatedSolinas.add_correct in H
-      | context [UnsaturatedSolinas.sub] =>
-        apply UnsaturatedSolinas.sub_correct in H
-      | context [UnsaturatedSolinas.opp] =>
-        apply UnsaturatedSolinas.opp_correct in H
-      | context [UnsaturatedSolinas.carry] =>
-        apply UnsaturatedSolinas.carry_correct in H
-      | context [UnsaturatedSolinas.encode] =>
-        apply UnsaturatedSolinas.encode_correct in H
-      | context [UnsaturatedSolinas.zero] =>
-        apply UnsaturatedSolinas.zero_correct in H
-      | context [UnsaturatedSolinas.one] =>
-        apply UnsaturatedSolinas.one_correct in H
-      | context [UnsaturatedSolinas.to_bytes] =>
-        apply UnsaturatedSolinas.to_bytes_correct in H
-      | context [UnsaturatedSolinas.from_bytes] =>
-        apply UnsaturatedSolinas.from_bytes_correct in H
-      end.
-
-    Ltac apply_correctness :=
-      match goal with H : _ = ErrorT.Success _ |- _ =>
-                      apply_correctness_in H;
-                      [ | assumption .. ]
-      end.
-
-    Record Op {t : API.type}
-          (pipeline_out : Pipeline.ErrorT (API.Expr t)) :=
-      { post :
-          type.for_each_lhs_of_arrow API.interp_type t ->
-          API.interp_type (type.base (type.final_codomain t)) -> Prop;
-        correctness :
-          check_args
-            n s c Semantics.width (ErrorT.Success tt) = ErrorT.Success tt ->
-          forall res,
-            pipeline_out = ErrorT.Success res ->
-            forall args,
-              post args (type.app_curried (API.Interp res) args) }.
-    Arguments post {_ _}.
-    Arguments correctness {_ _}.
-
-    Ltac specialize_to_args Hcorrect :=
-      let A := fresh "A" in
-      let A' := fresh "A" in
-      match goal with
-        a : type.for_each_lhs_of_arrow API.interp_type _ |- _ =>
-        cbn in a; set (A:=a)
-      end;
-      repeat match type of A with
-               (?xt * ?yt)%type =>
-               specialize (Hcorrect (fst A));
-               set (A':=snd A); subst A;
-               rename A' into A
-             end;
-      subst A.
-    Ltac instantiate_postcondition Hcorrect :=
-      let Ht := fresh "Ht" in
-      let G := fresh "G" in
-      match type of Hcorrect with ?T => set (Ht:=T) end;
-      match goal with |- ?g => set (G:=g) end;
-      repeat
-        (let g := (eval hnf in G) in
-         let E := fresh "E" in
-         match g with
-         | ?f ?e =>
-           remember e as E;
-           let T := (eval hnf in Ht) in
-           let y := lazymatch (eval pattern E in T) with
-                      ?f _ => f end in
-           let y := (eval cbn iota zeta delta in y) in
-           let Ht' := fresh "Ht" in
-           set (Ht':=y);
-           subst G; set (G:=f);
-           subst Ht; rename Ht' into Ht; subst E
-         end);
-      subst G;
-      let T := (eval hnf in Ht) in
-      instantiate (1:=T); exact Hcorrect.
-    Ltac pose_evar_for_post_with_name name :=
-      let T := fresh "T" in
-      let postT := fresh "postT" in
-      let postT' := fresh "postT" in
-      match goal with
-        |- @Op ?t _ => pose (T := t) end;
-      pose (postT := Prop);
-      repeat
-        (let t := (eval hnf in T) in
-         let bodyt := (eval hnf in postT) in
-         match t with
-         | type.arrow ?s ?d =>
-           let st := (eval cbn in (API.interp_type s)) in
-           rename postT into postT';
-           pose (postT := st -> postT'); subst postT' T;
-           pose (T:=d)
-         | ?s =>
-           let st := (eval cbn in (API.interp_type s)) in
-           rename postT into postT';
-           pose (postT := st -> postT'); subst postT' T
-         end);
-      evar (name : postT); subst postT.
-    Ltac prove_Op :=
-      repeat match goal with p := _ |- _ => subst p end;
-      intros;
-      let Hcorrect :=
-          lazymatch goal with
-            H : _ = ErrorT.Success _ |- _ => H end in
-      apply_correctness;
-      specialize_to_args Hcorrect;
-      fold weight in Hcorrect;
-      cbn; instantiate_postcondition Hcorrect.
-
-    Definition carry_mul_op
-      : Op (UnsaturatedSolinas.carry_mul n s c Semantics.width).
-    Proof.
-      pose_evar_for_post_with_name body.
-      (* TODO: below uncurrying of post could probably be automated (for other
-         ops as well) *)
-      apply Build_Op with
-          (post:= fun args =>
-                    let x := fst args in
-                    let y := fst (snd args) in
-                    body x y).
-      prove_Op.
-    Defined.
-
-    Definition add_op
-      : Op (UnsaturatedSolinas.add n s c Semantics.width).
-    Proof.
-      pose_evar_for_post_with_name body.
-      apply Build_Op with
-          (post:= fun args =>
-                    let x := fst args in
-                    let y := fst (snd args) in
-                    body x y).
-      prove_Op.
-    Defined.
-
-    Definition to_bytes_op
-      : Op (UnsaturatedSolinas.to_bytes n s c Semantics.width).
-    Proof.
-      pose_evar_for_post_with_name body.
-      apply Build_Op
-        with (post:= fun args =>
-                       let x := fst args in
-                       body x).
-      prove_Op.
-    Defined.
-
-    (* TODO: move *)
-    Definition within_input_sizes
-               {t} (sig : FunctionSignature t)
-               (args : type.for_each_lhs_of_arrow API.interp_type t) : Prop :=
-      LoadStoreList.within_access_sizes_args args sig.(input_array_sizes).
-    Definition within_output_sizes
-               {t} (sig : FunctionSignature t)
-               (out : base.interp (type.final_codomain t)) : Prop :=
-      LoadStoreList.within_base_access_sizes out sig.(output_array_sizes).
-    Definition output_sizes_obeyed
-               {t} (sig : FunctionSignature t) (res : API.Expr t) : Prop :=
-      forall args,
-        within_input_sizes sig args ->
-        within_output_sizes sig (type.app_curried (API.Interp res) args).
-
-    (* TODO: definition to construct seplogic/args automatically from type? Put in Op? *)
-    Definition spec_of_carry_mul : spec_of carry_mul_name :=
-      fun functions =>
-        forall wx wy px py pout wold_out t m
-               (Ra Rr : Semantics.mem -> Prop),
-          sep (sep (BignumSuchThat px wx (fun l => length l = n))
-                   (BignumSuchThat py wy (fun l => length l = n)))
-              Ra m ->
-          sep (BignumSuchThat pout wold_out (fun l => length l = n))
-              Rr m ->
-          let args := (map word.unsigned wx,
-                       (map word.unsigned wy, tt)) in
-          within_input_sizes carry_mul args ->
-          WeakestPrecondition.call
-            functions carry_mul_name t m
-            (px :: py :: pout :: nil)
-            (fun t' m' rets =>
-               t = t' /\
-               rets = []%list /\
-               exists wout,
-                 sep (BignumSuchThat pout wout (post carry_mul_op args))
-                     Rr m').
-
-    Definition spec_of_add : spec_of add_name :=
-      fun functions =>
-        forall wx wy px py pout wold_out t m
-               (Ra Rr : Semantics.mem -> Prop),
-          sep (sep (BignumSuchThat px wx (fun l => length l = n))
-                   (BignumSuchThat py wy (fun l => length l = n)))
-              Ra m ->
-          sep (BignumSuchThat pout wold_out (fun l => length l = n))
-              Rr m ->
-          let args := (map word.unsigned wx,
-                       (map word.unsigned wy, tt)) in
-          within_input_sizes add args ->
-          WeakestPrecondition.call
-            functions add_name t m
-            (px :: py :: pout :: nil)
-            (fun t' m' rets =>
-               t = t' /\
-               rets = []%list /\
-               exists wout,
-                 sep (BignumSuchThat pout wout (post add_op args))
-                     Rr m').
-
-    Definition spec_of_to_bytes : spec_of to_bytes_name :=
-      fun functions =>
-        forall wx px pout wold_out t m
-               (Ra Rr : Semantics.mem -> Prop),
-          sep (BignumSuchThat px wx (fun l => length l = n)) Ra m ->
-          sep (EncodedBignumSuchThat pout wold_out
-                                     (fun l => length l = n_bytes))
-              Rr m ->
-          let args := (map word.unsigned wx, tt) in
-          within_input_sizes to_bytes args ->
-          WeakestPrecondition.call
-            functions to_bytes_name t m
-            (px :: pout :: nil)
-            (fun t' m' rets =>
-               t = t' /\
-               rets = []%list /\
-               exists wout,
-                 sep (EncodedBignumSuchThat pout wout (post to_bytes_op args))
-                     Rr m').
-
     Context (check_args_ok :
                check_args n s c Semantics.width (ErrorT.Success tt)
                = ErrorT.Success tt).
 
-    Definition output_lengths_ok
-               {t} (sig : FunctionSignature t) (res : API.Expr t)
-      : Prop :=
-      forall args : type.for_each_lhs_of_arrow API.interp_type t,
-        LoadStoreList.list_lengths_from_value
-          (type.app_curried (API.Interp res) args)
-        = sig.(output_array_lengths).
-
     Definition is_correct
                {t : API.type}
                (start : Pipeline.ErrorT (API.Expr t))
-               (sig : FunctionSignature t)
+               (op : operation t)
                {name : string} (spec : spec_of name) : Prop :=
       (forall res : API.Expr t,
           start = ErrorT.Success res ->
           expr.Wf3 res ->
           valid_func (res (fun _ : API.type => unit)) ->
-          output_sizes_obeyed sig res ->
-          output_lengths_ok sig res ->
           forall functions,
-            spec (make_bedrock_func sig res :: functions)).
+            spec (make_bedrock_func op res :: functions)).
 
     Ltac setup :=
       match goal with
         |- is_correct _ ?def ?spec =>
-        cbv [is_correct def spec make_bedrock_func
-                        output_sizes_obeyed within_output_sizes
-                        within_input_sizes] in *; intros;
-        sepsimpl
+        cbv [is_correct spec make_bedrock_func] in *; intros;
+        sepsimpl;
+        cbn [def name inbounds input_array_sizes output_array_sizes
+                 input_array_lengths output_array_lengths
+                 pipeline_out correctness] in *
       end;
-      cbn [name input_array_sizes output_array_sizes] in *.
+      match goal with |- context [postcondition ?op ?args] =>
+                      let H := fresh in
+                      pose proof (correctness op) as H;
+                      repeat specialize (H ltac:(assumption));
+                      specialize (H args)
+      end; cleanup.
+
+    Ltac simplify_translate_func_postcondition :=
+      match goal with
+        H : context [sep _ _ ?m] |- context [_ ?m] =>
+        cbn - [Memory.bytes_per translate_func] in H
+      end;
+    sepsimpl_hyps.
+
+    Ltac ssubst :=
+      repeat match goal with
+             | H : literal (word.unsigned _) (eq _) |- _ =>
+               inversion H as [H']; clear H;
+               rewrite word.of_Z_unsigned in H'
+             | H : word.unsigned _ = word.unsigned _ |- _ =>
+               apply word.unsigned_inj in H
+             end; subst.
 
     Lemma carry_mul_correct :
       is_correct
@@ -528,53 +522,32 @@ Section __.
         carry_mul spec_of_carry_mul.
     Proof.
       setup.
-      match goal with |- context [post ?op ?args] =>
-                      pose proof (correctness op) (ltac:(assumption))
-                           ltac:(assumption) ltac:(assumption) args
-      end.
 
-      (* pick out arguments *)
-      match goal with |- context [post ?op ?args] =>
-                      set (A:=args) end.
-
-      (* get output length here for convenience *)
-      match goal with H : output_lengths_ok _ _ |- _ =>
-                      specialize (H A); cbn - [n_bytes] in H end.
+      (* TODO: put something to this effect in [operation] to make it more
+         uniform? *)
+      (* fetch output length for convenience *)
+      let out := lazymatch goal with
+                 | H : postcondition _ _ ?out |- _ => out end in
+      assert (length out = n)
+        by (apply bounded_by_loose_bounds_length; prove_bounds).
 
       (* TODO: automate flat_args, out_ptrs? *)
       (* use translate_func_correct to get the translation postcondition *)
+      let a := lazymatch goal with
+               | H : postcondition _ ?args _ |- _ => args end in
       eapply Proper_call;
         [ | eapply translate_func_correct with
                 (Ra0:=Ra) (Rr0:=Rr) (out_ptrs:=[pout])
-                (args:=A) (flat_args := [px; py]) ]; subst A.
-
+                (args:=a) (flat_args := [px; py]) ].
       { (* prove that the translation postcondition is sufficient *)
         repeat intro.
-        match goal with
-          H : context [sep _ _ ?m] |- context [_ ?m] =>
-          cbn - [Memory.bytes_per translate_func] in H
-        end.
-        sepsimpl_hyps; ssplit; [ congruence | congruence | eexists ].
-        fold Bignum in *.
+        simplify_translate_func_postcondition.
+        ssplit; [ congruence | congruence | eexists ].
+        cbn [type.app_curried fst snd] in *; cbv [expr.Interp] in *.
         sepsimpl;
-          [ erewrite map_unsigned_of_Z, map_word_wrap_bounded
-            by (eapply max_bounds_range_iff; eauto);
-            match goal with H : _ |- _ => apply H; assumption end | ].
-        cbv [Bignum expr.Interp].
-        match goal with
-        | H : literal (word.unsigned _) (eq _) |- _ =>
-          inversion H as [H']; clear H;
-            rewrite word.of_Z_unsigned in H'
-        end.
-        match goal with H : word.unsigned _ = word.unsigned _ |- _ =>
-                        apply word.unsigned_inj in H end.
-        (* TODO: without the below clear, subst fails, this is dumb *)
-        repeat match goal with H : _ = n |- _ => clear H end.
-        subst.
-        match goal with
-          H : map word.unsigned _ = ?l |- context [map word.of_Z ?l] =>
-          rewrite <-H, map_of_Z_unsigned
-        end.
+          [ match goal with H : map word.unsigned _ = _ |- _ =>
+                            rewrite H; solve [eauto] end | ].
+        ssubst. cbv [Bignum].
         rewrite word_size_in_bytes_eq.
         use_sep_assumption.
         rewrite array_truncated_scalar_scalar_iff1.
@@ -588,7 +561,9 @@ Section __.
            flatten_make_innames_NoDup, flatten_make_outnames_NoDup.
 
       { (* list lengths are correct *)
-        cbn. congruence. }
+        cbn.
+        rewrite !bounded_by_loose_bounds_length by prove_bounds.
+        reflexivity. }
       { (* arg pointers are correct *)
         cbn - [Memory.bytes_per]; sepsimpl.
         next_argument. exists_list_ptr px.
@@ -600,14 +575,22 @@ Section __.
       { (* input access sizes are legal *)
         pose proof bits_per_word_le_width.
         cbn - [Memory.bytes_per]; tauto. }
+      { (* input access sizes are accurate *)
+        cbn - [Memory.bytes_per]; ssplit; try tauto;
+          eapply max_bounds_range_iff; prove_bounds. }
       { (* output access sizes are legal *)
         pose proof bits_per_word_le_width.
         cbn - [Memory.bytes_per]; tauto. }
+      { (* output access sizes are accurate *)
+        cbn - [Memory.bytes_per].
+        eapply max_bounds_range_iff; prove_bounds. }
       { (* space is reserved for output lists *)
         cbn - [Memory.bytes_per]. sepsimpl.
-        cbv [expr.Interp] in *. cbn [Compilers.base_interp] in *.
+        cbv [expr.Interp] in *.
+        cbn [fst snd type.app_curried Compilers.base_interp] in *.
         exists (map word.unsigned wold_out).
-        sepsimpl; [ rewrite map_length in *; congruence | ].
+        sepsimpl;
+          [ rewrite map_length in *; congruence | ].
         exists pout; sepsimpl; [ ].
         eexists.
         sepsimpl; [ reflexivity
@@ -622,63 +605,42 @@ Section __.
                   | ].
         cbv [Bignum] in *.
         rewrite <-word_size_in_bytes_eq.
-        use_sep_assumption.
-        rewrite array_truncated_scalar_scalar_iff1.
-        cancel. }
+        repeat seprewrite array_truncated_scalar_scalar_iff1.
+        ecancel_assumption. }
     Qed.
+
     Lemma add_correct :
       is_correct
         (UnsaturatedSolinas.add n s c Semantics.width)
         add spec_of_add.
     Proof.
       setup.
-      match goal with |- context [post ?op ?args] =>
-                      pose proof (correctness op) (ltac:(assumption))
-                           ltac:(assumption) ltac:(assumption) args
-      end.
 
-      (* pick out arguments *)
-      match goal with |- context [post ?op ?args] =>
-                      set (A:=args) end.
-
-      (* get output length here for convenience *)
-      match goal with H : output_lengths_ok _ _ |- _ =>
-                      specialize (H A); cbn - [n_bytes] in H end.
+      (* TODO: put something to this effect in [operation] to make it more
+         uniform? *)
+      (* fetch output length for convenience *)
+      let out := lazymatch goal with
+                 | H : postcondition _ _ ?out |- _ => out end in
+      assert (length out = n)
+        by (apply bounded_by_loose_bounds_length; prove_bounds).
 
       (* TODO: automate flat_args, out_ptrs? *)
       (* use translate_func_correct to get the translation postcondition *)
+      let a := lazymatch goal with
+               | H : postcondition _ ?args _ |- _ => args end in
       eapply Proper_call;
         [ | eapply translate_func_correct with
                 (Ra0:=Ra) (Rr0:=Rr) (out_ptrs:=[pout])
-                (args:=A) (flat_args := [px; py]) ]; subst A.
-
+                (args:=a) (flat_args := [px; py]) ].
       { (* prove that the translation postcondition is sufficient *)
         repeat intro.
-        match goal with
-          H : context [sep _ _ ?m] |- context [_ ?m] =>
-          cbn - [Memory.bytes_per translate_func] in H
-        end.
-        sepsimpl_hyps; ssplit; [ congruence | congruence | eexists ].
-        fold Bignum in *.
+        simplify_translate_func_postcondition.
+        ssplit; [ congruence | congruence | eexists ].
+        cbn [type.app_curried fst snd] in *; cbv [expr.Interp] in *.
         sepsimpl;
-          [ erewrite map_unsigned_of_Z, map_word_wrap_bounded
-            by (eapply max_bounds_range_iff; eauto);
-            match goal with H : _ |- _ => apply H; assumption end | ].
-        cbv [Bignum expr.Interp].
-        match goal with
-        | H : literal (word.unsigned _) (eq _) |- _ =>
-          inversion H as [H']; clear H;
-            rewrite word.of_Z_unsigned in H'
-        end.
-        match goal with H : word.unsigned _ = word.unsigned _ |- _ =>
-                        apply word.unsigned_inj in H end.
-        (* TODO: without the below clear, subst fails, this is dumb *)
-        repeat match goal with H : _ = n |- _ => clear H end.
-        subst.
-        match goal with
-          H : map word.unsigned _ = ?l |- context [map word.of_Z ?l] =>
-          rewrite <-H, map_of_Z_unsigned
-        end.
+          [ match goal with H : map word.unsigned _ = _ |- _ =>
+                            rewrite H; solve [eauto] end | ].
+        ssubst. cbv [Bignum].
         rewrite word_size_in_bytes_eq.
         use_sep_assumption.
         rewrite array_truncated_scalar_scalar_iff1.
@@ -692,7 +654,9 @@ Section __.
            flatten_make_innames_NoDup, flatten_make_outnames_NoDup.
 
       { (* list lengths are correct *)
-        cbn. congruence. }
+        cbn.
+        rewrite !bounded_by_loose_bounds_length by prove_bounds.
+        reflexivity. }
       { (* arg pointers are correct *)
         cbn - [Memory.bytes_per]; sepsimpl.
         next_argument. exists_list_ptr px.
@@ -704,14 +668,22 @@ Section __.
       { (* input access sizes are legal *)
         pose proof bits_per_word_le_width.
         cbn - [Memory.bytes_per]; tauto. }
+      { (* input access sizes are accurate *)
+        cbn - [Memory.bytes_per]; ssplit; try tauto;
+          eapply max_bounds_range_iff; prove_bounds. }
       { (* output access sizes are legal *)
         pose proof bits_per_word_le_width.
         cbn - [Memory.bytes_per]; tauto. }
+      { (* output access sizes are accurate *)
+        cbn - [Memory.bytes_per].
+        eapply max_bounds_range_iff; prove_bounds. }
       { (* space is reserved for output lists *)
         cbn - [Memory.bytes_per]. sepsimpl.
-        cbv [expr.Interp] in *. cbn [Compilers.base_interp] in *.
+        cbv [expr.Interp] in *.
+        cbn [fst snd type.app_curried Compilers.base_interp] in *.
         exists (map word.unsigned wold_out).
-        sepsimpl; [ rewrite map_length in *; congruence | ].
+        sepsimpl;
+          [ rewrite map_length in *; congruence | ].
         exists pout; sepsimpl; [ ].
         eexists.
         sepsimpl; [ reflexivity
@@ -726,9 +698,8 @@ Section __.
                   | ].
         cbv [Bignum] in *.
         rewrite <-word_size_in_bytes_eq.
-        use_sep_assumption.
-        rewrite array_truncated_scalar_scalar_iff1.
-        cancel. }
+        repeat seprewrite array_truncated_scalar_scalar_iff1.
+        ecancel_assumption. }
     Qed.
 
     Lemma to_bytes_correct :
@@ -737,70 +708,70 @@ Section __.
         to_bytes spec_of_to_bytes.
     Proof.
       setup.
-      match goal with |- context [post ?op ?args] =>
-                      pose proof (correctness op) (ltac:(assumption))
-                           ltac:(assumption) ltac:(assumption) args
+
+      (* TODO: put something to this effect in [operation] to make it more
+         uniform? *)
+      (* fetch output length for convenience *)
+      (* differs from add/mul:
+        let out := lazymatch goal with
+                    | H : postcondition _ _ ?out |- _ => out end in
+        assert (length out = n)
+            by (apply bounded_by_loose_bounds_length; prove_bounds). *)
+      lazymatch goal with
+      | H : postcondition ?op _ ?out |- _ =>
+        assert (length out = n_bytes)
+          by (erewrite <-Partition.length_partition;
+              cbv [n_bytes limbwidth];
+              cbn [fst snd postcondition op] in H;
+              rewrite <-H by prove_bounds;
+              reflexivity)
       end.
 
-      (* pick out arguments *)
-      match goal with |- context [post ?op ?args] =>
-                      set (A:=args) end.
-
-      (* get output length here for convenience *)
-      match goal with H : output_lengths_ok _ _ |- _ =>
-                      specialize (H A); cbn - [n_bytes] in H end.
+      (* assert output bounds for convenience *)
+      match goal with
+      | H : postcondition ?op _ ?e |- _ =>
+        assert (list_Z_bounded_by (byte_bounds n_bytes) e)
+          by (cbn [fst snd postcondition op] in H;
+              rewrite H by prove_bounds;
+              apply partition_bounded_by)
+      end.
+      (* end differ *)
 
       (* TODO: automate flat_args, out_ptrs? *)
       (* use translate_func_correct to get the translation postcondition *)
+      (* differs from add/mul:
+        let a := lazymatch goal with
+                | H : postcondition _ ?args _ |- _ => args end in
+        eapply Proper_call;
+            [ | eapply translate_func_correct with
+                    (Ra0:=Ra) (Rr0:=Rr) (out_ptrs:=[pout])
+                    (args:=a) (flat_args := [px; py]) ]. *)
+      let a := lazymatch goal with
+               | H : postcondition _ ?args _ |- _ => args end in
       eapply Proper_call;
         [ | eapply translate_func_correct with
                 (Ra0:=Ra) (Rr0:=Rr) (out_ptrs:=[pout])
-                (args:=A) (flat_args := [px]) ]; subst A.
-
+                (args:=a) (flat_args := [px]) ].
       { (* prove that the translation postcondition is sufficient *)
         repeat intro.
-        match goal with
-          H : context [sep _ _ ?m] |- context [_ ?m] =>
-          cbn - [Memory.bytes_per translate_func] in H
-        end.
-        sepsimpl_hyps; ssplit; [ congruence | congruence | eexists ].
-        (* differs from mul/add *)
-        (* mul/add :
-           sepsimpl;
-             [ erewrite map_unsigned_of_Z, map_word_wrap_bounded
-               by (eapply max_bounds_range_iff; eauto);
-               match goal with H : _ |- _ => apply H; assumption end | ].
-        cbv [Bignum expr.Interp]. *)
+        simplify_translate_func_postcondition.
+        ssplit; [ congruence | congruence | eexists ].
+        cbn [type.app_curried fst snd] in *; cbv [expr.Interp] in *.
+        (* differs from add/mul:
+            sepsimpl;
+            [ match goal with H : map word.unsigned _ = _ |- _ =>
+                                rewrite H; solve [eauto] end | ].
+            ssubst. cbv [Bignum].
+            rewrite word_size_in_bytes_eq. *)
         sepsimpl;
           [ erewrite byte_map_unsigned_of_Z, map_byte_wrap_bounded
             by (eapply byte_bounds_range_iff; eauto);
             match goal with H : _ |- _ => apply H; assumption end | ].
-        cbv [EncodedBignum expr.Interp].
-        (* end differ *)
-        match goal with
-        | H : literal (word.unsigned _) (eq _) |- _ =>
-          inversion H as [H']; clear H;
-            rewrite word.of_Z_unsigned in H'
-        end.
-        match goal with H : word.unsigned _ = word.unsigned _ |- _ =>
-                        apply word.unsigned_inj in H end.
-        (* TODO: without the below clear, subst fails, this is dumb *)
-        repeat match goal with H : _ = n |- _ => clear H end.
-        subst.
-        (* differs from mul/add:
-        match goal with
-          H : map word.unsigned _ = ?l |- context [map word.of_Z ?l] =>
-          rewrite <-H, map_of_Z_unsigned
-        end.
-        rewrite word_size_in_bytes_eq.
-        use_sep_assumption.
-        rewrite array_truncated_scalar_scalar_iff1.
-        *)
-        subst.
-        match goal with
-          H : map word.unsigned _ = ?l |- context [?l] =>
-          rewrite <-H end.
+        ssubst. cbv [EncodedBignum].
         change (Z.of_nat (Memory.bytes_per access_size.one)) with 1 in *.
+        match goal with H : map word.unsigned _ = expr.interp _ _ _ |- _ =>
+                        rewrite <-H in * end.
+        (* end differ *)
         use_sep_assumption.
         rewrite array_truncated_scalar_ptsto_iff1.
         cancel. }
@@ -813,12 +784,15 @@ Section __.
            flatten_make_innames_NoDup, flatten_make_outnames_NoDup.
 
       { (* list lengths are correct *)
-        cbn. congruence. }
+        cbn.
+        rewrite !bounded_by_loose_bounds_length by prove_bounds.
+        reflexivity. }
       { (* arg pointers are correct *)
         cbn - [Memory.bytes_per]; sepsimpl.
         next_argument. exists_list_ptr px.
-        (* differs from mul/add:
-        next_argument. exists_list_ptr py. *)
+        (* differs from add/mul:
+            next_argument. exists_list_ptr py.
+         *)
         (* end differ *)
         cbv [Bignum] in *.
         repeat seprewrite array_truncated_scalar_scalar_iff1.
@@ -827,15 +801,25 @@ Section __.
       { (* input access sizes are legal *)
         pose proof bits_per_word_le_width.
         cbn - [Memory.bytes_per]; tauto. }
+      { (* input access sizes are accurate *)
+        cbn - [Memory.bytes_per]; ssplit; try tauto;
+          eapply max_bounds_range_iff; prove_bounds. }
       { (* output access sizes are legal *)
-        (* differs from mul/add :
-        pose proof bits_per_word_le_width.
-        cbn - [Memory.bytes_per]; tauto. *)
-        cbn. apply width_ge_8.
-        (* end differ *) }
+        (* differs from add/mul:
+            pose proof bits_per_word_le_width.
+            cbn - [Memory.bytes_per]; tauto. *)
+         cbn. apply width_ge_8. (* end differ *) }
+      { (* output access sizes are accurate *)
+        cbn - [Memory.bytes_per].
+        (* differs from add/mul:
+           cbv [expr.Interp] in *.
+           eapply max_bounds_range_iff; prove_bounds. *)
+        cbn [type.app_curried fst snd] in *. cbv [expr.Interp] in *.
+        eapply byte_bounds_range_iff. prove_bounds. (* end differ *)}
       { (* space is reserved for output lists *)
         cbn - [Memory.bytes_per]. sepsimpl.
-        cbv [expr.Interp] in *. cbn [Compilers.base_interp] in *.
+        cbv [expr.Interp] in *.
+        cbn [fst snd type.app_curried Compilers.base_interp] in *.
         (* differs from mul/add:
         exists (map word.unsigned wold_out). *)
         exists (map byte.unsigned wold_out).
@@ -864,18 +848,109 @@ Section __.
         (* differs from mul/add:
         cbv [Bignum] in *.
         rewrite <-word_size_in_bytes_eq.
-        use_sep_assumption.
-        rewrite array_truncated_scalar_scalar_iff1. *)
+        repeat seprewrite array_truncated_scalar_scalar_iff1. *)
         cbv [EncodedBignum] in *.
         rewrite map_unsigned_of_Z.
         erewrite map_word_wrap_bounded by
             auto using byte_unsigned_within_max_bounds.
         change (Z.of_nat (Memory.bytes_per access_size.one)) with 1 in *.
-        use_sep_assumption.
-        rewrite array_truncated_scalar_ptsto_iff1.
+        seprewrite array_truncated_scalar_ptsto_iff1.
         rewrite byte_map_of_Z_unsigned.
         (* end differ *)
-        cancel. }
+        ecancel_assumption. }
     Qed.
   End Proofs.
 End __.
+
+  (* TODO: delete if unused
+  Fixpoint word_base_interp (t : base.type) : Type :=
+    match t with
+    | base.type.prod a b => word_base_interp a * word_base_interp b
+    | base_listZ => list Semantics.word
+    | _ => Semantics.word
+    end.
+  Definition word_interp := type.interp word_base_interp.
+  Fixpoint ptr_base_interp (t : base.type) : Type :=
+    match t with
+    | base.type.prod a b => ptr_base_interp a * ptr_base_interp b
+    | _ => Semantics.word
+    end.
+  Definition ptr_interp := type.interp ptr_base_interp.
+
+  Fixpoint in_bounds {t}
+    : ZRange.type.base.option.interp t
+      -> ptr_base_interp t -> word_base_interp t
+      -> Semantics.mem -> Prop :=
+    match t with
+    | base.type.prod a b =>
+      fun bounds ptrs values =>
+        sep (in_bounds (fst bounds) (fst ptrs) (fst values))
+            (in_bounds (snd bounds) (snd ptrs) (snd values))
+    | base_listZ =>
+      fun bounds ptr value =>
+        match bounds with
+        | Some bounds =>
+          BignumSuchThat ptr value (list_Z_bounded_by bounds)
+        | None => emp False
+        end
+    | base_Z =>
+      fun bounds ptr value =>
+        sep (emp (ZRange.type.base.option.is_bounded_by
+                    bounds (word.unsigned value) = true))
+            (scalar ptr value)
+    | _ => fun _ _ _ => emp False
+    end.
+  Fixpoint input_ok {t}
+    : foreach_arg ZRange.type.option.interp t
+      -> foreach_arg ptr_interp t
+      -> foreach_arg word_interp t
+      -> Semantics.mem -> Prop :=
+    match t with
+    | type.base b => fun _ _ _ => emp True
+    | type.arrow (type.base s) d =>
+      fun bounds ptrs values =>
+        sep (in_bounds (fst bounds) (fst ptrs) (fst values))
+            (input_ok (snd bounds) (snd ptrs) (snd values))
+    | _ => fun _ _ _ => emp False
+    end.
+
+  (* What would be really nice:
+     In [operation], include
+        in_pre : foreach_arg ptr_interp t ->
+                 foreach_arg word_interp t ->
+                 Semantics.mem -> Prop
+        out_pre: foreach_ret ptr_interp t ->
+                 foreach_ret word_interp t ->
+    and use tactics to infer these
+
+    pros :
+         spec becomes very simple and duplicates across operations
+    cons:
+        makes spec harder to view/modify
+  *)
+
+  Fixpoint lengths_match {t}
+    : base_list_lengths t
+      -> ptr_base_interp t -> word_base_interp t
+      -> Semantics.mem -> Prop :=
+    match t with
+    | base.type.prod a b =>
+      fun lengths ptrs values =>
+        sep (lengths_match (fst lengths) (fst ptrs) (fst values))
+            (lengths_match (snd lengths) (snd ptrs) (snd values))
+    | base_listZ =>
+      fun n ptr value =>
+        BignumSuchThat ptr value (fun l => length l = n)
+    | base_Z =>
+      fun lengths ptr value =>
+        sep (emp (ZRange.type.base.option.is_bounded_by
+                    lengths (word.unsigned value) = true))
+            (scalar ptr value)
+    | _ => fun _ _ _ => emp False
+    end.
+  Definition output_placeholder_ok {t}
+    : foreach_ret list_lengths t
+      -> foreach_ret ptr_interp t
+      -> foreach_ret word_interp t
+      -> Semantics.mem -> Prop :=
+*)
